Tidying up Bit Machine and its proof of correctness.

Coq/Simplicity/BitMachine.v
@@ -1,26 +1,6 @@
 Require Import PeanoNat.
 Require Import List.
-
-Definition option_join {A} (x : option (option A)) : option A :=
-match x with
-| None => None
-| Some x => x
-end.
-
-Definition option_bind {A B} (f : A -> option B) (x : option A) : option B :=
-option_join (option_map f x).
-
-Lemma option_bind_ext {A B} (f1 f2 : A -> option B) :
-  (forall a, f1 a = f2 a) -> forall x, option_bind f1 x = option_bind f2 x.
-Proof.
-intros H [a|];[apply H|reflexivity].
-Qed.
-
-Lemma option_bind_assoc {A B C} (g : B -> option C) (f : A -> option B) x :
-  option_bind g (option_bind f x) = option_bind (fun a => option_bind g (f a)) x.
-Proof.
-destruct x as [a|];reflexivity.
-Qed.
+Require Import Util.Option.
 
 Definition Cell := option bool.
 
@@ -73,19 +53,31 @@ Notation "p ;; q" := (MachineCode.append p q) (at level 40, left associativity) 
 Definition nop : MachineCode.T := MachineCode.End.
 Definition bump n p : MachineCode.T := fwd n ;; p ;; bwd n.
 
+(* Write-only frames are append only.  We represent the frame by, writeData,
+ * the list of cells before the frame's cursor, and by writeEmpty, which
+ * contains the number of undefined cells after the cursor.
+ *
+ * The writeData store the list of cells in reverse order! This is analogous to
+ * the zipper used in ReadFrame below.
+ *)
 Record WriteFrame :=
  { writeData : list Cell
  ; writeEmpty : nat
- ; writeSize := length writeData + writeEmpty
  }.
 
-Definition newWriteFrame n : WriteFrame := Build_WriteFrame nil n.
-Definition fullWriteFrame l : WriteFrame := Build_WriteFrame (rev l) 0.
+Definition writeSize wf := length (writeData wf) + (writeEmpty wf).
+
+Definition newWriteFrame n : WriteFrame := {| writeData := nil; writeEmpty := n |}.
+
+(* Note that fullWriteFrame take a list of cells in forward order and
+ * transforms it into the reverse representation.
+ *)
+Definition fullWriteFrame l : WriteFrame := {| writeData := rev l; writeEmpty := 0 |}.
 
 Definition writeToFrame v f : option WriteFrame :=
 match writeEmpty f with
 | O => None
-| (S n) => Some (Build_WriteFrame (v :: writeData f) n)
+| (S n) => Some {| writeData := v :: writeData f; writeEmpty := n |}
 end.
 
 Fixpoint writeListFrame l f : option WriteFrame :=
@@ -94,28 +86,38 @@ match l with
 | hd :: tl => option_bind (writeListFrame tl) (writeToFrame hd f)
 end.
 
+(* Read-only frames are represented in zipper format.  The cells before the
+ * cursor are stored in prevData in reverse order.  The cells after the cursor
+ * are stored in nextData in forward order.
+ *)
 Record ReadFrame :=
  { prevData : list Cell
  ; nextData : list Cell
- ; readSize := length prevData + length nextData
  }.
+
+Definition readSize rf := length (prevData rf) + length (nextData rf).
+
+Definition setFrame l :=
+ {| prevData := nil
+  ; nextData := l
+  |}.
 
 Definition resetFrame wf :=
 match writeEmpty wf with
-| O => Some (Build_ReadFrame nil (rev (writeData wf)))
+| O => Some (setFrame (rev (writeData wf)))
 | S _ => None
 end.
 
 Definition advFrame f :=
 match nextData f with
 | nil => None
-| hd :: tl => Some (Build_ReadFrame (hd :: prevData f) tl)
+| hd :: tl => Some {| prevData := hd :: prevData f; nextData := tl |}
 end.
 
 Definition retFrame f :=
 match prevData f with
 | nil => None
-| hd :: tl => Some (Build_ReadFrame tl (hd :: nextData f))
+| hd :: tl => Some {| prevData := tl; nextData := hd :: nextData f |}
 end.
 
 Fixpoint fwdFrame n f :=
@@ -140,9 +142,8 @@ Lemma fwdFrame_correct l : forall pd nd,
  = Some {| prevData := rev l ++ pd; nextData := nd |}.
 Proof.
 induction l;[reflexivity|].
-simpl.
-unfold option_bind, advFrame; simpl.
 intros pd nd.
+cbn.
 rewrite IHl, <- app_assoc.
 reflexivity.
 Qed.
@@ -152,9 +153,8 @@ Lemma bwdFrame_correct l : forall pd nd,
  = Some {| prevData := pd; nextData := rev l ++ nd |}.
 Proof.
 induction l;[reflexivity|].
-simpl.
-unfold option_bind, retFrame; simpl.
 intros pd nd.
+cbn.
 rewrite IHl, <- app_assoc.
 reflexivity.
 Qed.
@@ -162,14 +162,11 @@ Qed.
 Lemma sliceFrame_correct l pd nd :
   sliceFrame (length l) {| prevData := pd; nextData := l ++ nd |} = Some l.
 Proof.
-unfold sliceFrame; simpl.
+unfold sliceFrame; cbn.
 rewrite app_length.
-case (Nat.leb_spec0 _ _).
- intros _.
- rewrite (plus_n_O (length l)), firstn_app_2, firstn_O, app_nil_r.
- reflexivity.
-intros [].
-auto with *.
+case (Nat.leb_spec0 _ _);[intros _|intros []; auto with *].
+rewrite (plus_n_O (length l)), firstn_app_2, firstn_O, app_nil_r.
+reflexivity.
 Qed.
 
 Definition readFromFrame f := hd None (nextData f).
@@ -177,65 +174,108 @@ Definition readFromFrame f := hd None (nextData f).
 Record ActiveFrames :=
  { readFrame : ReadFrame
  ; writeFrame : WriteFrame
- ; activeSize := readSize readFrame + writeSize writeFrame
  }.
 
+Definition activeSize af := readSize (readFrame af) + writeSize (writeFrame af).
+
 Definition oModReadFrame f act : option ActiveFrames :=
-  option_map (fun x => Build_ActiveFrames x (writeFrame act)) 
+  option_map (fun x => {| readFrame := x; writeFrame := writeFrame act |})
        (f (readFrame act)).
 
 Definition oModWriteFrame f act : option ActiveFrames :=
-  option_map (fun x => Build_ActiveFrames (readFrame act) x) 
+  option_map (fun x => {| readFrame := readFrame act; writeFrame := x |})
        (f (writeFrame act)).
 
+(* The full state of the Bit Machine is captured by a list of inactive
+ * read-only and write-only frames.  The top of the two stacks are held in the
+ * activeFrames.  This ensures that both stacks are non-empty.
+ *)
 Record State :=
  { inactiveReadFrames : list ReadFrame
  ; activeFrames : ActiveFrames
  ; inactiveWriteFrames : list WriteFrame
- ; stateSize := fold_right plus 0 (map readSize inactiveReadFrames) +
-                activeSize activeFrames +
-                fold_right plus 0 (map writeSize inactiveWriteFrames)
  }.
+
+Definition stateSize s :=
+  fold_right plus 0 (map readSize (inactiveReadFrames s)) +
+  activeSize (activeFrames s) +
+  fold_right plus 0 (map writeSize (inactiveWriteFrames s)).
 
 Definition oModActive f s : option State :=
-  option_map (fun x => Build_State (inactiveReadFrames s) x (inactiveWriteFrames s)) 
+  option_map (fun x => {| inactiveReadFrames := inactiveReadFrames s
+                        ; activeFrames := x
+                        ; inactiveWriteFrames := inactiveWriteFrames s
+                        |})
        (f (activeFrames s)).
 
+(* Logically, the state of the Bit Machine is commonly divided between the part
+ * of the state that we are focused on and the rest of state.  The focused part
+ * consists of some fragment of data after the cursor in the read-only frame,
+ * which contains the encoding of the input to some sub-expression in
+ * Simplicity, and some fragment of data around the cursor in the write-only
+ * frame, which contins the, partially written, output of some sub-expression.
+ *
+ * This focused part of the state is captured by the LocalState type.
+ * The remainder of the state is captured by the Context type, and happens to
+ * be isomorphic to the State type.  The fillContext function combines the
+ * LocalState with some context to produce a complete state.
+ *)
 Definition Context := State.
 
-Record Hole :=
- { readHole : list Cell
- ; writeHole : WriteFrame
+Definition emptyCtx : Context :=
+ {| inactiveReadFrames := nil
+  ; activeFrames :=
+    {| readFrame := setFrame nil
+     ; writeFrame := newWriteFrame 0
+     |}
+  ; inactiveWriteFrames := nil
+  |}.
+
+Record LocalState :=
+ { readLocalState : list Cell
+ ; writeLocalState : WriteFrame
  }.
 
-Definition fillContext (ctx : Context) (h : Hole) : State :=
+Definition fillContext (ctx : Context) (h : LocalState) : State :=
  {| inactiveReadFrames := inactiveReadFrames ctx
   ; activeFrames :=
     {| readFrame :=
       {| prevData := prevData (readFrame (activeFrames ctx))
-       ; nextData := readHole h ++ nextData (readFrame (activeFrames ctx))
+       ; nextData := readLocalState h ++ nextData (readFrame (activeFrames ctx))
        |}
      ; writeFrame :=
-      {| writeData := writeData (writeHole h) ++ writeData (writeFrame (activeFrames ctx))
-       ; writeEmpty := writeEmpty (writeHole h) + writeEmpty (writeFrame (activeFrames ctx))
+      {| writeData := writeData (writeLocalState h) ++ writeData (writeFrame (activeFrames ctx))
+       ; writeEmpty := writeEmpty (writeLocalState h) + writeEmpty (writeFrame (activeFrames ctx))
        |}
      |}
   ; inactiveWriteFrames := inactiveWriteFrames ctx
   |}.
 
-Definition appendHole (h1 h2 : Hole) : Hole :=
- {| readHole := readHole h2 ++ readHole h1
-  ; writeHole :=
-    {| writeData := writeData (writeHole h2) ++ writeData (writeHole h1)
-     ; writeEmpty := writeEmpty (writeHole h2) + writeEmpty (writeHole h1)
+(* Sometimes we need to focus in on part of the LocalState.  We can divide the
+ * LocalState into a localer state and its (relative) context.  Both the
+ * localer state and its context are isomorphic to the LocalState type and we
+ * do not give them separate types.
+ * We define appendLocalState to combine ls2, a LocalState representing the
+ * localer state, with ls1, a LocalState representing its relative context.
+ * Note that this append operation makes LocalState a monoid.
+ *)
+
+Definition appendLocalState (ls1 ls2 : LocalState) : LocalState :=
+ {| readLocalState := readLocalState ls2 ++ readLocalState ls1
+  ; writeLocalState :=
+    {| writeData := writeData (writeLocalState ls2) ++ writeData (writeLocalState ls1)
+     ; writeEmpty := writeEmpty (writeLocalState ls2) + writeEmpty (writeLocalState ls1)
      |}
   |}.
 
-Lemma context_action ctx h1 h2 :
-  fillContext (fillContext ctx h1) h2 = fillContext ctx (appendHole h1 h2).
+(* The monoid for LocalState above makes fillContext into a (right) monoid
+ * action on Contexts.
+ *)
+Lemma context_action ctx ls1 ls2 :
+  fillContext (fillContext ctx ls1) ls2 = fillContext ctx (appendLocalState ls1 ls2).
 Proof.
 unfold fillContext.
-simpl.
+cbn.
 repeat rewrite app_assoc.
 rewrite Plus.plus_assoc.
 reflexivity.
@@ -258,83 +298,70 @@ Definition fwd n :=
 Definition bwd n :=
   oModActive (oModReadFrame (bwdFrame n)).
 
-Definition newFrame n s := Some (Build_State
-   (inactiveReadFrames s)
-   (Build_ActiveFrames (readFrame (activeFrames s)) (newWriteFrame n))
-   (writeFrame (activeFrames s) :: inactiveWriteFrames s)).
+Definition newFrame n s :=
+  Some {| inactiveReadFrames := inactiveReadFrames s
+        ; activeFrames :=
+          {| readFrame := readFrame (activeFrames s)
+           ; writeFrame := newWriteFrame n
+           |}
+        ; inactiveWriteFrames := writeFrame (activeFrames s) :: inactiveWriteFrames s
+        |}.
 
 Definition moveFrame s :=
 match inactiveWriteFrames s with
 | nil => None
-| hd :: tl => option_map (fun x => Build_State
-  (readFrame (activeFrames s) :: inactiveReadFrames s)
-  (Build_ActiveFrames x hd)
-  tl) (resetFrame (writeFrame (activeFrames s)))
+| hd :: tl => option_map (fun x =>
+  {| inactiveReadFrames := readFrame (activeFrames s) :: inactiveReadFrames s
+   ; activeFrames :=
+     {| readFrame := x
+      ; writeFrame := hd
+      |}
+   ; inactiveWriteFrames := tl
+   |}) (resetFrame (writeFrame (activeFrames s)))
 end.
 
 Definition dropFrame s :=
 match inactiveReadFrames s with
 | nil => None
-| hd :: tl => Some (Build_State
-  tl
-  (Build_ActiveFrames hd (writeFrame (activeFrames s)))
-  (inactiveWriteFrames s))
+| hd :: tl => Some
+  {| inactiveReadFrames := tl
+   ; activeFrames :=
+     {| readFrame := hd
+      ; writeFrame := writeFrame (activeFrames s)
+      |}
+   ; inactiveWriteFrames := inactiveWriteFrames s
+   |}
 end.
 
 Lemma skip_correct n m l0 l1 (ctx : Context) :
-  skip n (fillContext ctx {| readHole := l0; writeHole := {| writeData := l1; writeEmpty := n + m |} |})
-= Some (fillContext ctx {| readHole := l0; writeHole := {| writeData := repeat None n ++ l1; writeEmpty := m |} |}).
+  skip n (fillContext ctx {| readLocalState := l0; writeLocalState := {| writeData := l1; writeEmpty := n + m |} |})
+= Some (fillContext ctx {| readLocalState := l0; writeLocalState := {| writeData := repeat None n ++ l1; writeEmpty := m |} |}).
 Proof.
-unfold skip.
-unfold oModActive.
-unfold oModWriteFrame.
-unfold fillContext.
-simpl.
+unfold skip, fillContext, oModActive, oModWriteFrame.
+cbn.
 revert l1.
 induction n;[reflexivity|].
 intros l1.
-simpl.
-unfold writeToFrame.
-simpl.
+cbn.
 set (wd := writeData (writeFrame (activeFrames ctx))).
 change (None :: (repeat None n ++ l1) ++ wd) with ((repeat None (S n) ++ l1) ++ wd).
-replace (repeat None (S n)) with (repeat (@None bool) n ++ (None :: nil)).
- rewrite <- (app_assoc _ _ l1).
- apply (IHn (None :: l1)).
-clear - n.
-induction n.
- reflexivity.
-simpl.
-f_equal.
-assumption.
+rewrite <- repeat_S_tail.
+rewrite <- (app_assoc _ _ l1).
+apply (IHn (None :: l1)).
 Qed.
 
 Lemma copy_correct (l : list Cell) (ctx : Context) :
-  copy (length l) (fillContext ctx {| readHole := l; writeHole := newWriteFrame (length l) |})
-= Some (fillContext ctx {| readHole := l; writeHole := fullWriteFrame l |}).
+  copy (length l) (fillContext ctx {| readLocalState := l; writeLocalState := newWriteFrame (length l) |})
+= Some (fillContext ctx {| readLocalState := l; writeLocalState := fullWriteFrame l |}).
 Proof.
-destruct ctx.
-unfold copy.
-unfold fillContext.
-unfold oModActive.
-simpl.
-rewrite sliceFrame_correct.
-unfold option_bind; simpl.
-set (rf := (Build_ReadFrame _ _)).
-generalize rf; clear rf; intros rf. (* TODO there is probably a tactic for this *)
-unfold oModWriteFrame; simpl.
-destruct activeFrames0. clear activeSize0 stateSize0.
-destruct writeFrame0 as [wd we _].
-simpl in *.
-revert wd;induction l;[reflexivity|];intros wd.
-simpl.
-unfold writeToFrame; simpl.
-unfold option_bind; simpl.
-rewrite IHl.
-rewrite <- app_assoc.
+unfold copy, fillContext, oModActive, oModWriteFrame; cbn.
+rewrite sliceFrame_correct; cbn.
+set (rf := (Build_ReadFrame _ _)); clearbody rf.
+set (wd := writeData _); clearbody wd; revert wd.
+induction l;[reflexivity|];intros wd; cbn.
+rewrite IHl, <- app_assoc.
 reflexivity.
 Qed.
-
 
 End State.
 
@@ -375,12 +402,12 @@ Definition bumpContext (ctx : Context) l : Context :=
   ; inactiveWriteFrames := inactiveWriteFrames ctx
   |}.
 
-Definition bumpHole l : Hole := {| readHole := l; writeHole := newWriteFrame 0 |}.
+Definition bumpLocalState l : LocalState := {| readLocalState := l; writeLocalState := newWriteFrame 0 |}.
 
-Lemma runMachine_bump ctx l h1 h2 p :
-    runMachine p (fillContext (bumpContext ctx l) h1) = Some (fillContext (bumpContext ctx l) h2)
- -> runMachine (bump (length l) p) (fillContext ctx (appendHole h1 (bumpHole l)))
-    = Some (fillContext ctx (appendHole h2 (bumpHole l))).
+Lemma runMachine_bump ctx l ls1 ls2 p :
+    runMachine p (fillContext (bumpContext ctx l) ls1) = Some (fillContext (bumpContext ctx l) ls2)
+ -> runMachine (bump (length l) p) (fillContext ctx (appendLocalState ls1 (bumpLocalState l)))
+    = Some (fillContext ctx (appendLocalState ls2 (bumpLocalState l))).
 Proof.
 intros Hp.
 unfold bump.
@@ -391,11 +418,10 @@ unfold State.fwd, oModActive, oModReadFrame.
 simpl (option_map _ _).
 rewrite <- app_assoc, fwdFrame_correct.
 unfold option_bind at 2; simpl (option_join _).
-change (runMachine p _) with (runMachine p (fillContext (bumpContext ctx l) h1)).
+change (runMachine p _) with (runMachine p (fillContext (bumpContext ctx l) ls1)).
 rewrite Hp.
-unfold option_bind; simpl.
-unfold State.bwd, oModActive, oModReadFrame.
-simpl.
+unfold option_bind; cbn.
+unfold State.bwd, oModActive, oModReadFrame; cbn.
 rewrite <- rev_length, bwdFrame_correct, rev_involutive, <- app_assoc.
 reflexivity.
 Qed.
