Coq/Util/List.v
@@ -1,0 +1,20 @@
+Require Export Coq.Lists.List.
+
+Lemma repeat_S_tail {A} : forall (a : A) n, repeat a n ++ (a :: nil) = repeat a (S n).
+Proof.
+intros a.
+induction n;[reflexivity|].
+simpl.
+rewrite IHn.
+reflexivity.
+Qed.
+
+Lemma rev_repeat {A} : forall (a : A) n, rev (repeat a n) = repeat a n.
+Proof.
+intros a.
+induction n;[reflexivity|].
+simpl.
+rewrite IHn, repeat_S_tail.
+reflexivity.
+Qed.
+
