Coq/Util/Option.v
@@ -1,0 +1,20 @@
+Definition option_join {A} (x : option (option A)) : option A :=
+match x with
+| None => None
+| Some x => x
+end.
+
+Definition option_bind {A B} (f : A -> option B) (x : option A) : option B :=
+option_join (option_map f x).
+
+Lemma option_bind_ext {A B} (f1 f2 : A -> option B) :
+  (forall a, f1 a = f2 a) -> forall x, option_bind f1 x = option_bind f2 x.
+Proof.
+intros H [|];[apply H|reflexivity].
+Qed.
+
+Lemma option_bind_assoc {A B C} (g : B -> option C) (f : A -> option B) x :
+  option_bind g (option_bind f x) = option_bind (fun a => option_bind g (f a)) x.
+Proof.
+destruct x as [|];reflexivity.
+Qed.
